Ever closer to full automation for binary encoders.

src/BinEncoders/Env/Common/Specs.v
@@ -110,6 +110,25 @@ Section Specifications.
 
 End Specifications.
 
+Lemma DecodeBindOpt2_assoc {A B C D E F G} :
+  forall (a_opt : option (A * B * D))
+         (f : A -> B -> D -> option (C * E * D))
+         (g : C -> E -> D -> option (F * G * D)),
+    DecodeBindOpt2 (DecodeBindOpt2 a_opt f) g =
+    DecodeBindOpt2 a_opt (fun a b c => DecodeBindOpt2 (f a b c) g).
+Proof.
+  destruct a_opt as [ [ [? ?] ?] | ]; simpl; intros; eauto.
+Qed.
+
+Lemma DecodeBindOpt2_under_bind {A B C D E} :
+  forall (a_opt : option (A * B * D))
+         (f f' : A -> B -> D -> option (C * E * D)),
+         (forall a b d, f a b d = f' a b d)
+         -> DecodeBindOpt2 a_opt f = DecodeBindOpt2 a_opt f'.
+Proof.
+  destruct a_opt as [ [ [? ?] ?] | ]; simpl; intros; eauto.
+Qed.
+
 Add Parametric Morphism
     A B
     (cache : Cache)
@@ -276,3 +295,35 @@ Notation "`( a , b ) <- c ; k" :=
 
 Open Scope binencoders_scope.
 Global Unset Implicit Arguments.
+
+Definition CorrectDecoderFor {A B} {cache : Cache}
+           {transformer : Transformer B} Invariant FormatSpec :=
+{ decodePlusCacheInv |
+      exists P_inv,
+        (cache_inv_Property (snd decodePlusCacheInv) P_inv
+         -> encode_decode_correct_f (A := A) cache transformer Invariant (fun _ _ => True)
+                                    FormatSpec
+                                    (fst decodePlusCacheInv)
+                                    (snd decodePlusCacheInv))
+        /\ cache_inv_Property (snd decodePlusCacheInv) P_inv}.
+
+Lemma Start_CorrectDecoderFor
+      {A B} {cache : Cache}
+      {transformer : Transformer B} Invariant FormatSpec
+      (decoder decoder_opt : B -> CacheDecode -> option (A * B * CacheDecode))
+      (cache_inv : CacheDecode -> Prop)
+      (P_inv : (CacheDecode -> Prop) -> Prop)
+      (decoder_OK : cache_inv_Property cache_inv P_inv
+         -> encode_decode_correct_f (A := A) cache transformer Invariant (fun _ _ => True)
+                                    FormatSpec decoder cache_inv)
+      (cache_inv_OK : cache_inv_Property cache_inv P_inv)
+      (decoder_opt_OK : forall b cd, decoder b cd = decoder_opt b cd)
+  : @CorrectDecoderFor A B cache transformer Invariant FormatSpec.
+Proof.
+  exists (decoder_opt, cache_inv); exists P_inv; split; simpl; eauto.
+  unfold encode_decode_correct_f in *; intuition; intros.
+  - destruct (H1 _ _ _ _ _ ext H0 H3 H4 H5).
+    rewrite decoder_opt_OK in H6; eauto.
+  - rewrite <- decoder_opt_OK in H4; destruct (H2 _ _ _ _ _ _ H0 H3 H4); eauto.
+  - rewrite <- decoder_opt_OK in H4; destruct (H2 _ _ _ _ _ _ H0 H3 H4); eauto.
+Defined.
