src/BinEncoders/Env/Examples/TCP_Packet.v
@@ -35,359 +35,255 @@ Open Scope string_scope.
 Open Scope Tuple_scope.
 
 (* Start Example Derivation. *)
+Section TCPPacketDecoder.
 
-Definition TCP_Packet :=
-  @Tuple <"SourcePort" :: word 16,
-          "DestPort" :: word 16,
-          "SeqNumber" :: word 32,
-          "AckNumber" :: word 32,
-          "NS" :: bool, (* ECN-nonce concealment protection flag *)
-          "CWR" :: bool, (* Congestion Window Reduced (CWR) flag *)
-          "ECE" :: bool, (* ECN-Echo flag *)
-          (* We can infer the URG flag from the Urgent Pointer field *)
-          "ACK" :: bool, (* Acknowledgment field is significant flag *)
-          "PSH" :: bool, (* Push function flag *)
-          "RST" :: bool, (* Reset the connection flag *)
-          "SYN" :: bool, (* Synchronize sequence numbers flag *)
-          "FIN" :: bool, (* No more data from sender flag*)
-          "WindowSize" :: word 16,
-          "UrgentPointer" :: option (word 16),
-          "Options" :: list (word 32),
-          "Payload" :: list char >.
+  Definition TCP_Packet :=
+    @Tuple <"SourcePort" :: word 16,
+    "DestPort" :: word 16,
+    "SeqNumber" :: word 32,
+    "AckNumber" :: word 32,
+    "NS" :: bool, (* ECN-nonce concealment protection flag *)
+    "CWR" :: bool, (* Congestion Window Reduced (CWR) flag *)
+    "ECE" :: bool, (* ECN-Echo flag *)
+    (* We can infer the URG flag from the Urgent Pointer field *)
+    "ACK" :: bool, (* Acknowledgment field is significant flag *)
+    "PSH" :: bool, (* Push function flag *)
+    "RST" :: bool, (* Reset the connection flag *)
+    "SYN" :: bool, (* Synchronize sequence numbers flag *)
+    "FIN" :: bool, (* No more data from sender flag*)
+    "WindowSize" :: word 16,
+    "UrgentPointer" :: option (word 16),
+    "Options" :: list (word 32),
+    "Payload" :: list char >.
 
-Definition TCP_Checksum_Valid
-           (srcAddr : word 32)
-           (destAddr : word 32)
-           (tcpLength : word 16)
-           (n : nat)
-           (b : ByteString)
-  := IPChecksum_Valid (96 + n)
-                (transform (transform (encode_word srcAddr)
-                (transform (encode_word destAddr)
-                (transform (encode_word (wzero 8))
-                (transform (encode_word (natToWord 8 6))
-                           (encode_word tcpLength)))))
-                b).
+  (* These values are provided by the IP header for checksum calculation.*)
 
-Definition encode_TCP_Packet_Spec
-           (srcAddr : word 32)
-           (destAddr : word 32)
-           (tcpLength : word 16)
-           (* These values are provided by the IP header for checksum calculation.*)
-           (tcp : TCP_Packet) :=
-          (encode_word_Spec (tcp!"SourcePort")
-    ThenC encode_word_Spec (tcp!"DestPort")
-    ThenC encode_word_Spec (tcp!"SeqNumber")
-    ThenC encode_word_Spec (tcp!"AckNumber")
-    ThenC encode_nat_Spec 4 (5 + |tcp!"Options"|)
-    ThenC encode_unused_word_Spec 3 (* These bits are reserved for future use. *)
-    ThenC encode_bool_Spec tcp!"NS"
-    ThenC encode_bool_Spec tcp!"CWR"
-    ThenC encode_bool_Spec tcp!"ECE"
-    ThenC encode_bool_Spec (match tcp!"UrgentPointer" with
-                            | Some _ => true
-                            | _ => false
-                            end)
-    ThenC encode_bool_Spec tcp!"ACK"
-    ThenC encode_bool_Spec tcp!"PSH"
-    ThenC encode_bool_Spec tcp!"RST"
-    ThenC encode_bool_Spec tcp!"SYN"
-    ThenC encode_bool_Spec tcp!"FIN"
-    ThenC encode_word_Spec tcp!"WindowSize" DoneC)
-    ThenChecksum (TCP_Checksum_Valid srcAddr destAddr tcpLength) OfSize 16
-    ThenCarryOn (encode_option_Spec encode_word_Spec (encode_unused_word_Spec' 16 ByteString_id) tcp!"UrgentPointer"
-    ThenC encode_list_Spec encode_word_Spec tcp!"Options"
-    ThenC encode_list_Spec encode_word_Spec tcp!"Payload" DoneC).
+  Variable srcAddr : word 32.
+  Variable destAddr : word 32.
+  Variable tcpLength : word 16.
 
-Definition TCP_Packet_OK (tcpLength : word 16) (tcp : TCP_Packet) :=
-  lt (|tcp!"Options"|) 11
-  /\ wordToNat tcpLength = 20 (* length of packet header *)
-                 + (4 * |tcp!"Options"|) (* length of option field *)
-                 + (|tcp!"Payload"|).
+  Definition TCP_Checksum_Valid
+             (n : nat)
+             (b : ByteString)
+    := IPChecksum_Valid (96 + n)
+       (transform (transform (encode_word srcAddr)
+                  (transform (encode_word destAddr)
+                  (transform (encode_word (wzero 8))
+                  (transform (encode_word (natToWord 8 6))
+                  (encode_word tcpLength)))))
+                  b).
 
-Definition TCP_Packet_decoder'
-  : { decodePlusCacheInv |
-      forall srcAddr destAddr tcpLength,
-      exists P_inv,
-        (cache_inv_Property (snd decodePlusCacheInv) P_inv
-         -> encode_decode_correct_f _ transformer (TCP_Packet_OK tcpLength) (fun _ _ => True)
-                                    (encode_TCP_Packet_Spec srcAddr destAddr tcpLength)
-                                    ((fst decodePlusCacheInv) srcAddr destAddr tcpLength)
-                                    (snd decodePlusCacheInv))
-        /\ cache_inv_Property (snd decodePlusCacheInv) P_inv}.
-Proof.
-  start_synthesizing_decoder.
-  normalize_compose transformer.
-  unfold encode_TCP_Packet_Spec; pose_string_ids.
-  let p := (eval unfold Domain in
-               (fun tcp : TCP_Packet =>
-                  (tcp!StringId,
-                   (tcp!StringId0,
-                   (tcp!StringId1,
-                   (tcp!StringId2,
-                   (|tcp!StringId13|,
-                   (tcp!StringId3,
-                   (tcp!StringId4,
-                   (tcp!StringId5,
-                   (match tcp!StringId12 with
-                            | Some _ => true
-                            | _ => false
-                            end,
-                   (tcp!StringId6,
-                   (tcp!StringId7,
-                   (tcp!StringId8,
-                   (tcp!StringId9,
-                   (tcp!StringId10,
-                    tcp!StringId11
-           )))))))))))))))) in
-  let p := eval simpl in p in
-      eapply (@compose_IPChecksum_encode_correct_dep
-                TCP_Packet
-                _
-                _
-                _
-                _ _ _ H
-                p
-                (TCP_Packet_OK tcpLength)
-                _ _ _
-                (fun data' =>
-                   (encode_word_Spec (fst data')
-              ThenC encode_word_Spec (fst (snd data'))
-              ThenC encode_word_Spec (fst (snd (snd data')))
-              ThenC encode_word_Spec (fst (snd (snd (snd data'))))
-              ThenC encode_nat_Spec 4 (5 + (fst (snd (snd (snd (snd data'))))))
-              ThenC encode_unused_word_Spec 3 (* These bits are reserved for future use. *)
-              ThenC encode_bool_Spec (fst (snd (snd (snd (snd (snd data'))))))
-              ThenC encode_bool_Spec (fst (snd (snd (snd (snd (snd (snd data')))))))
-              ThenC encode_bool_Spec (fst (snd (snd (snd (snd (snd (snd (snd data'))))))))
-              ThenC encode_bool_Spec (fst (snd (snd (snd (snd (snd (snd (snd (snd data')))))))))
-              ThenC encode_bool_Spec (fst (snd (snd (snd (snd (snd (snd (snd (snd (snd data'))))))))))
-              ThenC encode_bool_Spec (fst (snd (snd (snd (snd (snd (snd (snd (snd (snd (snd data')))))))))))
-              ThenC encode_bool_Spec (fst (snd (snd (snd (snd (snd (snd (snd (snd (snd (snd (snd data'))))))))))))
-              ThenC encode_bool_Spec (fst (snd (snd (snd (snd (snd (snd (snd (snd (snd (snd (snd (snd data')))))))))))))
-              ThenC encode_bool_Spec (fst (snd (snd (snd (snd (snd (snd (snd (snd (snd (snd (snd (snd (snd data'))))))))))))))
-              ThenC encode_word_Spec (snd (snd (snd (snd (snd (snd (snd (snd (snd (snd (snd (snd (snd (snd data')))))))))))))) DoneC))).
-    simpl transform; unfold encode_word;
-    rewrite !ByteString_enqueue_ByteString_measure,
-    !length_encode_word';
-    reflexivity.
-  reflexivity.
-  repeat calculate_length_ByteString.
-  repeat calculate_length_ByteString.
-  solve_mod_8.
-  solve_mod_8.
-  { (* Grossest Proof By Far. *)
-    intros; change transform_id with ByteString_id; rewrite length_ByteString_ByteString_id.
-    instantiate (1 := fun _ => (wordToNat tcpLength) * 8);
-      cbv beta.
-    unfold TCP_Packet_OK in H2.
-    rewrite (proj2 H2).
-    unfold StringId13, StringId14.
+  Definition encode_TCP_Packet_Spec
+             (tcp : TCP_Packet) :=
+         (      encode_word_Spec (tcp!"SourcePort")
+          ThenC encode_word_Spec (tcp!"DestPort")
+          ThenC encode_word_Spec (tcp!"SeqNumber")
+          ThenC encode_word_Spec (tcp!"AckNumber")
+          ThenC encode_nat_Spec 4 (5 + |tcp!"Options"|)
+          ThenC encode_unused_word_Spec 3 (* These bits are reserved for future use. *)
+          ThenC encode_bool_Spec tcp!"NS"
+          ThenC encode_bool_Spec tcp!"CWR"
+          ThenC encode_bool_Spec tcp!"ECE"
+          ThenC encode_bool_Spec (match tcp!"UrgentPointer" with
+                                  | Some _ => true
+                                  | _ => false
+                                  end)
+          ThenC encode_bool_Spec tcp!"ACK"
+          ThenC encode_bool_Spec tcp!"PSH"
+          ThenC encode_bool_Spec tcp!"RST"
+          ThenC encode_bool_Spec tcp!"SYN"
+          ThenC encode_bool_Spec tcp!"FIN"
+          ThenC encode_word_Spec tcp!"WindowSize" DoneC)
+ThenChecksum (TCP_Checksum_Valid) OfSize 16
+ThenCarryOn (encode_option_Spec encode_word_Spec (encode_unused_word_Spec' 16 ByteString_id) tcp!"UrgentPointer"
+       ThenC encode_list_Spec encode_word_Spec tcp!"Options"
+       ThenC encode_list_Spec encode_word_Spec tcp!"Payload" DoneC).
+
+  Definition TCP_Packet_OK (tcp : TCP_Packet) :=
+    lt (|tcp!"Options"|) 11
+    /\ wordToNat tcpLength = 20 (* length of packet header *)
+                             + (4 * |tcp!"Options"|) (* length of option field *)
+                             + (|tcp!"Payload"|).
+
+  Local Arguments NPeano.modulo : simpl never.
+
+  Definition TCP_Packet_decoder'
+    : CorrectDecoderFor TCP_Packet_OK encode_TCP_Packet_Spec.
+  Proof.
+    start_synthesizing_decoder.
+    normalize_compose transformer.
+    eapply compose_IPChecksum_encode_correct_dep';
+      [ apply H
+      | repeat resolve_Checksum
+        | cbv beta; unfold Domain; simpl;
+            simpl transform; unfold encode_word;
+              rewrite !ByteString_enqueue_ByteString_measure,
+              !length_encode_word';
+              reflexivity
+        | cbv beta; unfold Domain; simpl; reflexivity
+        | cbv beta; unfold Domain; simpl;
+            repeat calculate_length_ByteString
+        | cbv beta; unfold Domain; simpl;
+            repeat calculate_length_ByteString
+        | cbv beta; unfold Domain; simpl;
+            solve_mod_8
+        | solve_mod_8
+        | .. ].
+    { (* Grossest Proof By Far. *)
+      unfold Domain; simpl.
+      intros; change transform_id with ByteString_id; rewrite length_ByteString_ByteString_id.
+      instantiate (1 := fun _ => (wordToNat tcpLength) * 8);
+        cbv beta.
+      unfold TCP_Packet_OK in H2.
+      rewrite (proj2 H2).
+      unfold StringId13, StringId14.
+      clear.
+      repeat match goal with
+               |- context [ @length ?A (@GetAttribute ?heading ?z ?l)] => remember (@length A (@GetAttribute heading z l))
+             end.
+      assert (n0 = n1) by (subst; reflexivity).
+      rewrite H.
+      omega.
+    }
+    unfold Domain; simpl.
+    decode_step.
+    decode_step.
+    decode_step.
+    decode_step.
+    decode_step.
+    decode_step.
+    decode_step.
+    decode_step.
+    decode_step.
+    decode_step.
+    decode_step.
+    decode_step.
+    decode_step.
+    decode_step.
+    decode_step.
+    decode_step.
+    decode_step.
+    decode_step.
+    decode_step.
+    decode_step.
+    decode_step.
+    decode_step.
+    decode_step.
+    decode_step.
+    decode_step.
+    decode_step.
+    decode_step. (* intros; eapply bool_decode_correct. *)
+
+    decode_step.
+    decode_step.
+    decode_step.
+    decode_step.
+    decode_step.
+    decode_step.
+    decode_step.
+    decode_step.
+    decode_step.
+    decode_step.
+    decode_step.
+    decode_step.
+    decode_step.
+    decode_step.
+    decode_step.
+    decode_step.
+    decode_step.
+    decode_step.
+    decode_step.
+    decode_step.
+    decode_step.
+    decode_step.
+    decode_step.
+    decode_step.
+
+    decode_step.
+    decode_step.
+    decode_step.
+    decode_step.
+    decode_step.
+    decode_step.
+
+    decode_step.
+    decode_step.
+    decode_step.
+    decode_step.
+    decode_step.
+    decode_step.
+    decode_step.
+    decode_step.
+    decode_step.
+
+    unfold TCP_Packet_OK; intros ? H'; repeat split.
+    simpl; destruct H'.
+    unfold pow2; simpl in *.
+    unfold GetAttribute, GetAttributeRaw in H0; simpl in H0.
+    revert H0; clear; unfold StringId13; intros; omega.
+
+    instantiate (1 := fun _ _ => True);
+      simpl; intros; exact I.
+
+    decode_step.
+    decode_step.
+    decode_step.
+    decode_step.
+    simpl; intros; split_and.
+    instantiate (1 := fst (snd (snd (snd (snd (snd (snd (snd (snd proj))))))))).
+    repeat match goal with
+             H : prod _ _ |- _ => destruct H
+           end.
+    simpl in *; injections.
+    match goal with
+      |- context [decides (negb match ?b with _ => _ end) (?b' = None) ] =>
+      assert (b = b') as H' by reflexivity; rewrite H'; destruct b';
+        simpl; intuition eauto
+    end.
+    discriminate.
+    destruct a'; intros; exact I.
+
+    decode_step.
+    decode_step.
+    decode_step.
+
+    simpl; intros; instantiate (1 := fst (snd (snd (snd (snd proj))))).
+    intuition; subst; simpl; auto with arith.
+    simpl in *.
+    clear; admit.
+
+    decode_step.
+    decode_step.
+    decode_step.
+    decode_step.
+    simpl in *; intros.
+    unfold TCP_Packet_OK in H3.
+    do 4 destruct H3.
+    split; eauto.
+    instantiate (1 := (wordToNat tcpLength) - 20 - (4 * fst (snd (snd (snd (snd proj)))))).
+    rewrite <- H6.
+    rewrite H7.
+    unfold snd, fst.
+    fold StringId14; fold StringId13.
     clear.
     repeat match goal with
              |- context [ @length ?A (@GetAttribute ?heading ?z ?l)] => remember (@length A (@GetAttribute heading z l))
            end.
     assert (n = n1) by (subst; reflexivity).
-    assert (n0 = n2) by (subst; reflexivity).
-    rewrite H, H0.
-    omega.
-  }
-  decode_step.
-  decode_step.
-  decode_step.
-  decode_step.
-  decode_step.
-  decode_step.
-  decode_step.
-  decode_step.
-  decode_step.
-  decode_step.
-  decode_step.
-  decode_step.
-  decode_step.
-  decode_step.
-  decode_step.
-  decode_step.
-  decode_step.
-  decode_step.
-  decode_step.
-  decode_step.
-  decode_step.
-  decode_step.
-  decode_step.
-  decode_step.
-  decode_step.
-  decode_step.
-  decode_step. (* intros; eapply bool_decode_correct. *)
+    rewrite H.
+    clear; admit.
 
-  decode_step.
-  decode_step.
-  decode_step.
-  decode_step.
-  decode_step.
-  decode_step.
-  decode_step.
-  decode_step.
-  decode_step.
-  decode_step.
-  decode_step.
-  decode_step.
-  decode_step.
-  decode_step.
-  decode_step.
-  decode_step.
-  decode_step.
-  decode_step.
-  decode_step.
-  decode_step.
-  decode_step.
-  decode_step.
-  decode_step.
-  decode_step.
+    decode_step.
 
-  decode_step.
-  decode_step.
-  decode_step.
-  decode_step.
-  decode_step.
-  decode_step.
+    intros; eapply encode_decode_correct_finish.
+    build_fully_determined_type.
+    decide_data_invariant.
+    synthesize_cache_invariant.
+    optimize_decoder_impl.
 
-  decode_step.
-  decode_step.
-  decode_step.
-  decode_step.
-  decode_step.
-  decode_step.
-  decode_step.
-  decode_step.
-  intros; eapply encode_decode_correct_finish.
+    Time Defined.
 
-  let a' := fresh in
-  intros a'; repeat destruct a' as [? a'].
-    (* Show that it is determined by the constraints (equalities) *)
-    (* inferred during parsing. *)
-  unfold GetAttribute, GetAttributeRaw in *;
-  simpl in *; intros;
-    (* Decompose data predicate *) intuition.
-  (* need to clean this up as well *)
-  assert (proj3 - 5 = n) as H' by omega; rewrite <- H'; clear H' H30.
-  subst.
-  reflexivity.
+  Definition TCP_Packet_decoder_impl :=
+    Eval simpl in (fst (projT1 TCP_Packet_decoder')).
 
-  decide_data_invariant.
-
-  unfold TCP_Packet_OK; clear; intros ? H'; repeat split.
-  simpl; destruct H'.
-  revert H; unfold pow2; simpl; clear.
-  unfold StringId13; intros; omega.
-  instantiate (1 := fun _ _ => True);
-    simpl; intros; exact I.
-
-  decode_step.
-  decode_step.
-  decode_step.
-  decode_step.
-  simpl; intros; split_and.
-  instantiate (1 := fst (snd (snd (snd (snd (snd (snd (snd (snd proj))))))))).
-  repeat match goal with
-           H : prod _ _ |- _ => destruct H
-         end.
-  simpl in *; injections.
-  match goal with
-    |- context [decides (negb match ?b with _ => _ end) (?b' = None) ] =>
-    assert (b = b') as H' by reflexivity; rewrite H'; destruct b';
-      simpl; intuition eauto
-  end.
-  discriminate.
-  destruct a'; intros; exact I.
-
-  decode_step.
-  decode_step.
-  decode_step.
-
-  simpl; intros; instantiate (1 := fst (snd (snd (snd (snd proj))))).
-  intuition; subst; simpl; auto with arith.
-  decode_step.
-  decode_step.
-  decode_step.
-  decode_step.
-  simpl in *; intros.
-  unfold TCP_Packet_OK in H3.
-  do 4 destruct H3.
-  split; eauto.
-  instantiate (1 := (wordToNat tcpLength) - 20 - (4 * fst (snd (snd (snd (snd proj)))))).
-  rewrite <- H6.
-  rewrite H7.
-  unfold snd, fst.
-  fold StringId14; fold StringId13.
-  clear.
-  repeat match goal with
-           |- context [ @length ?A (@GetAttribute ?heading ?z ?l)] => remember (@length A (@GetAttribute heading z l))
-         end.
-  assert (n = n1) by (subst; reflexivity).
-  assert (n0 = n2) by (subst; reflexivity).
-  rewrite H, H0.
-  omega.
-  decode_step.
-
-  intros; eapply encode_decode_correct_finish.
-
-    let a' := fresh in
-  intros a'; repeat destruct a' as [? a'].
-    (* Show that it is determined by the constraints (equalities) *)
-    (* inferred during parsing. *)
-  unfold GetAttribute, GetAttributeRaw in *;
-    simpl in *; intros;
-    (* Decompose data predicate *) intuition.
-  rename H14 into H17.
-  let H' := fresh in
-  pose proof (f_equal fst H17) as H'; simpl in H';
-    apply (f_equal snd) in H17; simpl in H17.
-  let H' := fresh in
-  pose proof (f_equal fst H17) as H'; simpl in H';
-    apply (f_equal snd) in H17; simpl in H17.
-  let H' := fresh in
-  pose proof (f_equal fst H17) as H'; simpl in H';
-    apply (f_equal snd) in H17; simpl in H17.
-  let H' := fresh in
-  pose proof (f_equal fst H17) as H'; simpl in H';
-    apply (f_equal snd) in H17; simpl in H17.
-  let H' := fresh in
-  pose proof (f_equal fst H17) as H'; simpl in H';
-    apply (f_equal snd) in H17; simpl in H17.
-  let H' := fresh in
-  pose proof (f_equal fst H17) as H'; simpl in H';
-    apply (f_equal snd) in H17; simpl in H17.
-  let H' := fresh in
-  pose proof (f_equal fst H17) as H'; simpl in H';
-    apply (f_equal snd) in H17; simpl in H17.
-  let H' := fresh in
-  pose proof (f_equal fst H17) as H'; simpl in H';
-    apply (f_equal snd) in H17; simpl in H17.
-  let H' := fresh in
-  pose proof (f_equal fst H17) as H'; simpl in H';
-    apply (f_equal snd) in H17; simpl in H17.
-  let H' := fresh in
-  pose proof (f_equal fst H17) as H'; simpl in H';
-    apply (f_equal snd) in H17; simpl in H17.
-  let H' := fresh in
-  pose proof (f_equal fst H17) as H'; simpl in H';
-    apply (f_equal snd) in H17; simpl in H17.
-  let H' := fresh in
-  pose proof (f_equal fst H17) as H'; simpl in H';
-    apply (f_equal snd) in H17; simpl in H17.
-  let H' := fresh in
-  pose proof (f_equal fst H17) as H'; simpl in H';
-    apply (f_equal snd) in H17; simpl in H17.
-  let H' := fresh in
-  pose proof (f_equal fst H17) as H'; simpl in H';
-    apply (f_equal snd) in H17; simpl in H17.
-  subst; reflexivity.
-  decide_data_invariant.
-  synthesize_cache_invariant.
-Time Defined.
-
-(*Definition TCP_Packet_decoder_impl :=
-  Eval simpl in (fst (projT1 TCP_Packet_decoder')).
-
-Print TCP_Packet_decoder_impl. *)
+Print TCP_Packet_decoder_impl.
