src/BinEncoders/Env/Examples/ARPPacket.v
@@ -34,42 +34,6 @@ Open Scope Tuple_scope.
 Opaque pow2. (* Don't want to be evaluating this. *)
 Opaque natToWord. (* Or this. *)
 
-Ltac apply_compose :=
-  intros;
-  match goal with
-    H : cache_inv_Property ?P ?P_inv |- _ =>
-    first [eapply (compose_encode_correct_no_dep H); clear H
-          | eapply (compose_encode_correct H); clear H
-          | eapply (composeIf_encode_correct H); clear H;
-            [ |
-              | solve [intros; intuition (eauto with bin_split_hints) ]
-              | solve [intros; intuition (eauto with bin_split_hints) ] ]
-          ]
-  end.
-
-Ltac makeEvar T k :=
-  let x := fresh in evar (x : T); let y := eval unfold x in x in clear x; k y.
-
-Ltac shelve_inv :=
-  let H' := fresh in
-  let data := fresh in
-  intros data H';
-  repeat destruct H';
-  match goal with
-  | H : ?P data |- ?P_inv' =>
-    is_evar P;
-    let P_inv' := (eval pattern data in P_inv') in
-    let P_inv := match P_inv' with ?P_inv data => P_inv end in
-    let new_P_T := type of P in
-    makeEvar new_P_T
-             ltac:(fun new_P =>
-                     unify P (fun data => new_P data /\ P_inv data)); apply (Logic.proj2 H)
-  end.
-
-Ltac solve_data_inv :=
-    first [ simpl; intros; exact I
-| shelve_inv ].
-
 Definition transformer : Transformer ByteString := ByteStringQueueTransformer.
 
 (* Start Example Derivation. *)
@@ -135,21 +99,9 @@ Definition ARP_Packet_OK (arp : ARPPacket) :=
 Arguments Vector.nth : simpl never.
 
 Definition ARPPacket_decoder
-  : { decodePlusCacheInv |
-      exists P_inv,
-      (cache_inv_Property (snd decodePlusCacheInv) P_inv
-       -> encode_decode_correct_f _ transformer ARP_Packet_OK (fun _ b => True)
-                                  encode_ARPPacket_Spec
-                                  (fst decodePlusCacheInv) (snd decodePlusCacheInv))
-      /\ cache_inv_Property (snd decodePlusCacheInv) P_inv}.
+  : CorrectDecoderFor ARP_Packet_OK encode_ARPPacket_Spec.
 Proof.
-  start_synthesizing_decoder.
-  repeat decode_step.
-  intros; simpl; intuition; subst; assumption.
-  intros; simpl; intuition; subst; try assumption.
-  intros; simpl; intuition; subst; assumption.
-  intros; simpl; intuition; subst; assumption.
-  synthesize_cache_invariant.
+  synthesize_decoder.
 Defined.
 
 Definition ARP_Packet_decoder :=
