src/BinEncoders/Env/Examples/EthernetHeader.v
@@ -37,119 +37,117 @@ Opaque natToWord. (* Or this. *)
 Definition transformer : Transformer ByteString := ByteStringQueueTransformer.
 
 (* Start Example Derivation. *)
+Section EthernetPacketDecoder.
 
-Definition EthernetHeader :=
-  @Tuple <"Destination" :: Vector.t char 6,
-  "Source" :: Vector.t char 6,
-  "Type" :: EnumType ["ARP"; "IP"; "RARP"]>.
+  Definition EthernetHeader :=
+    @Tuple <"Destination" :: Vector.t char 6,
+    "Source" :: Vector.t char 6,
+    "Type" :: EnumType ["ARP"; "IP"; "RARP"]>.
 
-Definition EtherTypeCodes : Vector.t (word 16) 3 :=
-  [WO~0~0~0~0~1~0~0~0~0~0~0~0~0~0~0~0;
-   WO~0~0~0~0~1~0~0~0~0~0~0~0~0~1~1~0;
-   WO~0~0~0~0~1~0~0~0~0~0~1~1~0~1~0~1
-  ].
+  Definition EtherTypeCodes : Vector.t (word 16) 3 :=
+    [WO~0~0~0~0~1~0~0~0~0~0~0~0~0~0~0~0;
+       WO~0~0~0~0~1~0~0~0~0~0~0~0~0~1~1~0;
+       WO~0~0~0~0~1~0~0~0~0~0~1~1~0~1~0~1
+    ].
 
-Definition encode_EthernetHeader_Spec n' (eth : EthernetHeader) :=
-          encode_Vector_Spec encode_word_Spec eth!"Destination"
-    ThenC (encode_Vector_Spec encode_word_Spec eth!"Source")
-    ThenC Either
-          encode_nat_Spec 16 n'
-          ThenC encode_word_Spec (WO~0~1~0~1~0~1~0~1)
-          ThenC encode_word_Spec (WO~0~1~0~1~0~1~0~1)
-          ThenC encode_word_Spec (WO~1~1~0~0~0~0~0~0)
-          ThenC encode_word_Spec (wzero 24)
-          ThenC encode_enum_Spec EtherTypeCodes eth!"Type"
-          DoneC
-       Or encode_enum_Spec EtherTypeCodes eth!"Type"
-          DoneC.
+  Variable packet_len : nat. (* The length of the ethernet packet, *)
+  (* which is a parameter to the encoder and decoder. *)
+  Variable packet_len_OK : lt packet_len 1501.
 
-Definition ethernet_Header_OK (e : EthernetHeader) := True.
+  Definition encode_EthernetHeader_Spec (eth : EthernetHeader) :=
+    encode_Vector_Spec encode_word_Spec eth!"Destination"
+                       ThenC (encode_Vector_Spec encode_word_Spec eth!"Source")
+                       ThenC Either
+                       encode_nat_Spec 16 packet_len
+                       ThenC encode_word_Spec (WO~0~1~0~1~0~1~0~1)
+                       ThenC encode_word_Spec (WO~0~1~0~1~0~1~0~1)
+                       ThenC encode_word_Spec (WO~1~1~0~0~0~0~0~0)
+                       ThenC encode_word_Spec (wzero 24)
+                       ThenC encode_enum_Spec EtherTypeCodes eth!"Type"
+                       DoneC
+                       Or encode_enum_Spec EtherTypeCodes eth!"Type"
+                       DoneC.
 
-Definition v1042_test (b : ByteString) : bool :=
-  match transformer_get_word 16 b with
-  | Some w => if wlt_dec w (natToWord 16 1501) then true else false
-  | _ => false
-  end.
+  Definition ethernet_Header_OK (e : EthernetHeader) := True.
 
-Lemma v1042_OKT
-  : forall n (data : EthernetHeader) (bin : ByteString) (env xenv : CacheEncode) (ext : ByteString),
-    lt n 1501 ->
-   (encode_nat_Spec 16 n
-    ThenC encode_word_Spec WO~0~1~0~1~0~1~0~1
-    ThenC encode_word_Spec WO~0~1~0~1~0~1~0~1
-    ThenC encode_word_Spec WO~1~1~0~0~0~0~0~0
-    ThenC encode_word_Spec (wzero 24) ThenC encode_enum_Spec EtherTypeCodes data!"Type" DoneC) env
-   ↝ (bin, xenv) -> v1042_test (transform bin ext) = true.
-Proof.
-  intros.
-  unfold compose at 1 in H0; unfold Bind2 in H0;
-    computes_to_inv; destruct v; destruct v0; simpl in *;
+  Definition v1042_test (b : ByteString) : bool :=
+    match transformer_get_word 16 b with
+    | Some w => if wlt_dec w (natToWord 16 1501) then true else false
+    | _ => false
+    end.
+
+  Lemma v1042_OKT
+    : forall (data : EthernetHeader) (bin : ByteString) (env xenv : CacheEncode) (ext : ByteString),
+      (encode_nat_Spec 16 packet_len
+                       ThenC encode_word_Spec WO~0~1~0~1~0~1~0~1
+                       ThenC encode_word_Spec WO~0~1~0~1~0~1~0~1
+                       ThenC encode_word_Spec WO~1~1~0~0~0~0~0~0
+                       ThenC encode_word_Spec (wzero 24) ThenC encode_enum_Spec EtherTypeCodes data!"Type" DoneC) env
+                                                                                                                  ↝ (bin, xenv) -> v1042_test (transform bin ext) = true.
+  Proof.
+    intros.
+    unfold compose at 1 in H; unfold Bind2 in H;
+      computes_to_inv; destruct v; destruct v0; simpl in *;
         injections.
-  unfold encode_nat_Spec, encode_word_Spec in H0; computes_to_inv.
-  pose proof (f_equal fst H0) as H'; simpl in H'; rewrite <- H'.
-  pose proof transform_assoc as H''; simpl in H''; rewrite <- H''.
-  unfold v1042_test.
-  pose transformer_get_encode_word' as H'''; rewrite H'''; find_if_inside; eauto.
-  destruct n0.
-  eapply natToWord_wlt; eauto; try reflexivity.
-  etransitivity.
-  unfold BinNat.N.lt; rewrite <- Nnat.Nat2N.inj_compare.
-  eapply Compare_dec.nat_compare_lt; eassumption.
-  reflexivity.
-Qed.
+    unfold encode_nat_Spec, encode_word_Spec in H; computes_to_inv.
+    pose proof (f_equal fst H) as H''; simpl in H''; rewrite <- H''.
+    pose proof transform_assoc as H'''; simpl in H'''; rewrite <- H'''.
+    unfold v1042_test.
+    pose transformer_get_encode_word' as H''''; rewrite H''''; find_if_inside; eauto.
+    destruct n.
+    eapply natToWord_wlt; eauto; try reflexivity.
+    etransitivity.
+    unfold BinNat.N.lt; rewrite <- Nnat.Nat2N.inj_compare.
+    eapply Compare_dec.nat_compare_lt; eassumption.
+    reflexivity.
+  Qed.
 
-Hint Resolve v1042_OKT : bin_split_hints.
+  Hint Resolve v1042_OKT : bin_split_hints.
 
-Lemma v1042_OKE
-  : forall (data : EthernetHeader) (bin : ByteString) (env xenv : CacheEncode) (ext : ByteString),
-    (encode_enum_Spec EtherTypeCodes data!"Type" DoneC) env ↝ (bin, xenv)
-    -> v1042_test (transform bin ext) = false.
-Proof.
-  intros; unfold compose at 1 in H; unfold Bind2 in H;
-    computes_to_inv; destruct v; destruct v0; simpl in *;
-      injections.
-  unfold encode_enum_Spec, encode_word_Spec in H; computes_to_inv.
-  pose proof (f_equal fst H) as H'; unfold fst in H'; rewrite <- H'.
-  pose proof transform_assoc as H''; simpl in H''; rewrite <- H''.
-  unfold v1042_test.
-  pose transformer_get_encode_word' as H'''; rewrite H'''; find_if_inside; eauto.
-  revert w; clear.
-  match goal with
-    |- context [Vector.nth (m := ?n) ?w ?idx] => remember idx; clear
-  end.
-  Local Transparent natToWord.
-  eapply forall_Vector_P; repeat econstructor;
-    unfold wlt; compute; intros; discriminate.
-Qed.
+  Lemma v1042_OKE
+    : forall (data : EthernetHeader) (bin : ByteString) (env xenv : CacheEncode) (ext : ByteString),
+      (encode_enum_Spec EtherTypeCodes data!"Type" DoneC) env ↝ (bin, xenv)
+      -> v1042_test (transform bin ext) = false.
+  Proof.
+    intros; unfold compose at 1 in H; unfold Bind2 in H;
+      computes_to_inv; destruct v; destruct v0; simpl in *;
+        injections.
+    unfold encode_enum_Spec, encode_word_Spec in H; computes_to_inv.
+    pose proof (f_equal fst H) as H'; unfold fst in H'; rewrite <- H'.
+    pose proof transform_assoc as H''; simpl in H''; rewrite <- H''.
+    unfold v1042_test.
+    pose transformer_get_encode_word' as H'''; rewrite H'''; find_if_inside; eauto.
+    revert w; clear.
+    match goal with
+      |- context [Vector.nth (m := ?n) ?w ?idx] => remember idx; clear
+    end.
+    Local Transparent natToWord.
+    eapply forall_Vector_P; repeat econstructor;
+      unfold wlt; compute; intros; discriminate.
+  Qed.
 
-Hint Resolve v1042_OKE : bin_split_hints.
+  Hint Resolve v1042_OKE : bin_split_hints.
 
-Lemma valid_packet_len_OK_good_Len
-    : forall packet_len,
-    lt packet_len 1501 -> lt packet_len (pow2 16).
+  Lemma valid_packet_len_OK_good_Len
+    : lt packet_len (pow2 16).
   Proof.
     intros.
     etransitivity; eauto.
     rewrite <- (wordToNat_natToWord_idempotent 16 1501).
     eapply wordToNat_bound.
     simpl; eapply BinNat.N.ltb_lt; reflexivity.
-Qed.
+  Qed.
 
   Hint Resolve valid_packet_len_OK_good_Len : data_inv_hints.
 
-Definition EthernetHeader_decoder
-  : { decodePlusCacheInv |
-      forall packet_len,
-        lt packet_len 1501
-        -> exists P_inv,
-          (cache_inv_Property (snd decodePlusCacheInv) P_inv
-           -> encode_decode_correct_f _ transformer ethernet_Header_OK (fun _ b => b = ByteString_id)
-                                      (encode_EthernetHeader_Spec packet_len)
-                                      (fst decodePlusCacheInv packet_len) (snd decodePlusCacheInv))
-          /\ cache_inv_Property (snd decodePlusCacheInv) P_inv}.
-Proof.
-  synthesize_decoder.
-Defined.
+  Definition EthernetHeader_decoder
+    : CorrectDecoderFor ethernet_Header_OK encode_EthernetHeader_Spec.
+  Proof.
+    synthesize_decoder.
+  Defined.
 
-Definition frame_decoder := Eval simpl in proj1_sig EthernetHeader_decoder.
+  Definition frame_decoder := Eval simpl in proj1_sig EthernetHeader_decoder.
+
+End EthernetPacketDecoder.
+
 Print frame_decoder.
